

Bayes' theorem tells us how to update our beliefs
(about unknown parameters, θ) w/ data.

in this class

$$p(\theta) \longrightarrow p(\theta | y)$$

\downarrow
 unknown parameter of the data generative model.

\nearrow data

$$p(\theta | y) = \frac{\overbrace{p(y | \theta)}^{\text{likelihood}} \overbrace{p(\theta)}^{\text{prior}}}{\int p(y | \theta) p(\theta) d\theta}$$

\downarrow
posterior

\downarrow constant: $\int p(y, \theta) d\theta = p(y)$

"marginal likelihood"

not a function of θ !

Typical scenario for a (Bayesian) Statistician:


here's a data set: 0, 1, 0, 0, ...

) Ask yourself: what simple model could have generated this data
obvious answer here: "binary" model: $x_i | \theta \stackrel{iid}{\sim} \text{binary}(\theta)$

i.e. $p(x_i = 1) = \theta$
 $p(x_i = 0) = (1 - \theta)$ and $\theta \in [0, 1]$

$$\Rightarrow p(x_1, \dots, x_n | \theta) = \theta^{\sum x_i} (1 - \theta)^{n - \sum x_i}$$

- always start w/ simplest model
- when in doubt, go to distr. sheet & look at support of various distributions.
- ... how likely they could have generated your data?

2) I identify what you don't know in the likelihood. 

Here : $\boxed{\theta}$

and write down a prior for all unknowns (consider the support of θ).

Candidate priors:

- $\text{Unif}(0,1)$
- $\text{beta}(a,b)$
- truncated normal

we'll begin by considering the uniform:

$$p(\theta) = \begin{cases} 1 & \text{if } \theta \in [0, 1] \\ 0 & \text{otherwise} \end{cases}$$

Together with our likelihood:

$$p(y|\theta) = \binom{n}{y} \theta^y (1-\theta)^{n-y}$$

← re-written as binomial according to transform

$$y = \sum_{i=1}^n x_i$$

we can directly write down our posterior (it is deterministically defined by likelihood & prior)

$$P(\theta|y) = \frac{\binom{n}{y} \theta^y (1-\theta)^{n-y} \cdot 1_{\{\theta \in [0,1]\}}}{p(y)}$$

But notice:

But notice:

$p(\theta|y) \propto \theta^y (1-\theta)^{n-y} \quad \theta \in [0,1]$

↑
proportional
in θ

This is the kernel of a beta(x, y) $x = y + 1$
 $y = n - x + 1$

Prove claim: beta prior is conjugate to binomial data generative model. (5)

In other words, show that

$$\theta \sim \text{beta}(a, b)$$

$$y|\theta \sim \text{binomial}(n, \theta)$$

implies $\theta|y \sim \text{beta}(\alpha, \beta)$ for some α, β .

Note: if we show that the posterior is proportional to the kernel of a beta density, we will be done.

Proof

$$\begin{aligned} p(\theta|y) &\propto \text{likelihood} \cdot \text{prior} \\ &\propto \theta^y (1-\theta)^{n-y} \cdot \theta^{a-1} (1-\theta)^{b-1} \\ &\propto \theta^{y+a-1} (1-\theta)^{(n-y+b)-1} \end{aligned}$$

$$\Rightarrow \theta|y \sim \text{beta}(y+a, n-y+b)$$

□

Exercise

show that for $\theta|y \sim \text{beta}(y+a, n-y+b)$

$$\lim_{n \rightarrow \infty} \mathbb{E}[\theta|y] = \bar{x} \quad \text{where } \bar{x} = \frac{1}{n} \sum x_i$$

proof

$$\mathbb{E}[\theta|y] = \frac{a+y}{a+b+n}, \quad \text{notice } y = n\bar{x},$$

$$\lim_{n \rightarrow \infty} \frac{a + n\bar{x}}{a+b+n} = \lim_{n \rightarrow \infty} \underbrace{\frac{a}{a+b+n}}_0 + \frac{n\bar{x}}{a+b+n} \cdot \frac{1/n}{1/n} = \frac{\bar{x}}{1} = \bar{x}$$

□